@prefix xsd: <http://www.w3.org/2001/XMLSchema#> .
@prefix owl: <http://www.w3.org/2002/07/owl#> .
@prefix xml: <http://www.w3.org/XML/1998/namespace> .
@prefix rdf: <http://www.w3.org/1999/02/22-rdf-syntax-ns#> .
@prefix rdfs: <http://www.w3.org/2000/01/rdf-schema#> .
@prefix skos: <http://www.w3.org/2004/02/skos/core#> .
@prefix dc: <http://purl.org/dc/elements/1.1/> .
@prefix dcterms: <http://purl.org/dc/terms/> .
@prefix voaf: <http://purl.org/vocommons/voaf#> .
@prefix vann: <http://purl.org/vocab/vann/> .
@prefix cc: <http://creativecommons.org/ns#> .

#################################################################
# Ontology
#################################################################

<http://example.org/sdmx-mm> a owl:Ontology, voaf:Vocabulary ;
    dc:title "A vocabulary for representing SDMX metadata"@en ;
    dc:creator "Franck Cotton" ;
    vann:preferredNamespacePrefix "sdmx-mm" ;
    vann:preferredNamespaceUri <http://example.org/sdmx-mm#> ;
    cc:license <http://creativecommons.org/licenses/by/4.0/> ;
    voaf:classNumber "2"^^xsd:integer ;
    voaf:propertyNumber "6"^^xsd:integer ;
    owl:versionInfo "Version 0.1 - 2017-02-04" .


#################################################################
# Classes
#################################################################

# RDF property corresponding to the SDMX metadata attribute

sdmx-mm:MetadataAttributeProperty a rdfs:Class, owl:Class;
    rdfs:label "Metadata attribute"@en;
    rdfs:comment "Defines a specific type of metadata."@en;
    rdfs:subClassOf rdf:Property;
    rdfs:isDefinedBy <http://example.org/sdmx-mm>.

# Specification related to a metadata attribute

sdmx-mm:MetadataAttributeSpecification a rdfs:Class, owl:Class;
    rdfs:label "Metadata attribute specification"@en;
    rdfs:comment "Used to define properties of a metadata attribute which are specific to its usage in an MSD."@en;
    rdfs:isDefinedBy <http://example.org/sdmx-mm>.

# RDF property corresponding to the SDMX metadata target

sdmx-mm:MetadataTarget a rdfs:Class, owl:Class;
    rdfs:label "Metadata target"@en;
    rdfs:comment "Defines a part of a data or metadata set to which the metadata is attached."@en;
    rdfs:isDefinedBy <http://example.org/sdmx-mm>.


#################################################################
# Data properties
#################################################################

# Presentational attributes are used to structure a report and do not have values

sdmx-mm:isPresentational a rdf:Property, owl:DatatypeProperty;
    rdfs:label "is presentational"@en;
    rdfs:comment "When true, indicates that an attribute is for presentation purpose only and cannot have a value by itself."@en;
    rdfs:domain sdmx-mm:MetadataAttributeSpecification;
    rdfs:range xsd:boolean;
    rdfs:isDefinedBy <http://example.org/sdmx-mm>.

# Indicates the order of the attributes in the report

sdmx-mm:order a rdf:Property, owl:DatatypeProperty;
    rdfs:label "order"@en;
    rdfs:comment "Indicates a priority order for the attributes of metadata sets with this structure."@en;
    rdfs:domain sdmx-mm:MetadataAttributeSpecification;
    rdfs:range xsd:int;
    rdfs:isDefinedBy <http://example.org/sdmx-mm>.

# Maximum number of occurrences of the attribute in a given context

sdmx-mm:minOccurs a rdf:Property, owl:DatatypeProperty;
    rdfs:label "minOccurs"@en;
    rdfs:comment "Specifies the minimum number of occurrences of the metadata attribute that may be reported at this point in the metadata report."@en;
    rdfs:domain sdmx-mm:MetadataAttributeSpecification;
    rdfs:range xsd:int;
    rdfs:isDefinedBy <http://example.org/sdmx-mm>.

# Maximum number of occurrences of the attribute in a given context

sdmx-mm:maxOccurs a rdf:Property, owl:DatatypeProperty;
    rdfs:label "maxOccurs"@en;
    rdfs:comment "Specifies the maximum number of occurrences of the metadata attribute that may be reported at this point in the metadata report."@en;
    rdfs:domain sdmx-mm:MetadataAttributeSpecification;
    rdfs:range xsd:int;
    rdfs:isDefinedBy <http://example.org/sdmx-mm>.


#################################################################
# Object properties
#################################################################

# Links a metadata attribute specification to its metadata attribute

sdmx-mm:metadataAttributeProperty a rdf:Property, owl:ObjectProperty;
    rdfs:label "metadata attribute"@en;
    rdfs:comment "Indicates a metadata attribute property associated to the metadata attribute specification."@en;
    rdfs:domain sdmx-mm:MetadataAttributeSpecification;
    rdfs:range sdmx-mm:MetadataAttributeProperty;
    rdfs:isDefinedBy <http://example.org/sdmx-mm>.

# Links a metadata attribute to its parent in the report structure

sdmx-mm:parent a rdf:Property, owl:ObjectProperty;
    rdfs:label "parent"@en;
    rdfs:comment "Associates a metadata attribute to its parent in the report."@en;
    rdfs:domain sdmx-mm:MetadataAttributeSpecification;
    rdfs:range sdmx-mm:MetadataAttributeSpecification;
    rdfs:isDefinedBy <http://example.org/sdmx-mm>.

# Links a metadata attribute to the associated concept

sdmx-mm:concept a rdf:Property, owl:ObjectProperty;
    rdfs:label "concept"@en;
    rdfs:comment "Gives the metadata concept associated to a MetadataAttributeProperty."@en;
    rdfs:domain sdmx-mm:MetadataAttributeProperty;
    rdfs:range skos:Concept;
    rdfs:isDefinedBy <http://example.org/sdmx-mm>.

# Links a metadata target to a target object that is part of its specification

sdmx-mm:targetObject a rdf:Property, owl:ObjectProperty;
    rdfs:label "target object"@en;
    rdfs:comment "Indicates a target object that is part of the metadata target definition."@en;
    rdfs:domain sdmx-mm:MetadataTarget;
    rdfs:isDefinedBy <http://example.org/sdmx-mm>.
